Examples/Imp.thy
@@ -1,0 +1,225 @@
+theory Imp
+  imports "../MergeSemTc/Seq" "../Semantics/Gensyn_Sem" "../MergeableTc/MergeableAList"
+          "../MergeableTc/Mergeable" "../MergeableTc/MergeableInstances"
+          "../Lifting/LiftUtils" "../Lifting/LiftInstances" "PrintCalcSeq"
+begin
+
+(* conditional/boolean expressions *)
+datatype cond_syn' =
+  Seqz
+  | Sltz
+  | Sgtz
+  | Sskip_cond
+
+type_synonym cond_state' = "bool * int"
+
+definition cond_sem :: "cond_syn' \<Rightarrow> cond_state' \<Rightarrow> cond_state'" where
+"cond_sem x s =
+  (case s of (b, i) \<Rightarrow>
+    (case x of
+      Seqz \<Rightarrow> ((i = 0), i)
+      | Sltz \<Rightarrow> ((i < 0), i)
+      | Sgtz \<Rightarrow> ((i > 0), i)
+      | Sskip_cond \<Rightarrow> s))"
+
+(* Imp control
+- IF
+- WHILE
+- SKIP
+*)
+
+datatype syn' =
+  Sif
+  | Sskip
+  | Swhile
+
+(* TODO: fix this so we can actually reassociate, the way you would
+   actually want to write it *)
+type_synonym state' = "(gensyn_skel * unit gs_result * dir) * bool"
+
+definition imp_ctl_sem :: "syn' \<Rightarrow> state' \<Rightarrow> state'" where
+"imp_ctl_sem x st =
+  (case st of ((sk, GRPath cp, d), b) \<Rightarrow>
+    (case x of
+      Sskip \<Rightarrow> st
+      | Sif \<Rightarrow> 
+        (case d of
+         Down \<Rightarrow> ((sk, GRPath (cp @ [0]), Down), b)
+         | Up xcp \<Rightarrow>
+                 (case get_suffix cp xcp of
+                    Some (xcph#xcpt) \<Rightarrow>
+                      (case xcph of
+                          0 \<Rightarrow> \<comment> \<open>condition\<close>
+                            (if b 
+                             then ((sk, GRPath (cp @ [1]), Down), b)
+                             else ((sk, GRPath (cp @ [2]), Down), b))
+                          | _ \<Rightarrow> \<comment> \<open> then/else \<close>
+                              (case gensyn_cp_parent sk cp of
+                                None \<Rightarrow> ((sk, GRDone, Up cp), b)
+                                | Some cp' \<Rightarrow> ((sk, GRPath cp', Up cp), b)))))
+        | Swhile \<Rightarrow>
+          (case d of
+           Down \<Rightarrow> ((sk, GRPath (cp @ [0]), Down), b)
+           | Up xcp \<Rightarrow>
+                 (case get_suffix cp xcp of
+                    Some (xcph#xcpt) \<Rightarrow>
+                      (case xcph of
+                          0 \<Rightarrow> \<comment> \<open>condition\<close>
+                            (if b 
+                             then ((sk, GRPath (cp @ [1]), Down), b)
+                             else (case gensyn_cp_parent sk cp of
+                                     None \<Rightarrow> ((sk, GRDone, Up cp), b)
+                                     | Some cp' \<Rightarrow> ((sk, GRPath cp', Up cp), b)))
+                          | _ \<Rightarrow> \<comment> \<open> loop body\<close>
+                              ((sk, GRPath cp, Down), b))))))"
+
+datatype syn = 
+  Spc PrintCalcSeq.syn
+  | Simp syn'
+  | Scond cond_syn'
+
+type_synonym state = 
+  "Seq.state * (bool md_triv option md_prio * PrintCalc.state)"
+
+definition imp_trans :: "syn \<Rightarrow> syn'" where
+"imp_trans s =
+  (case s of
+    Simp s' \<Rightarrow> s'
+    | _ \<Rightarrow> Sskip)"
+
+definition printcalc_trans :: "syn \<Rightarrow> PrintCalcSeq.syn" where
+"printcalc_trans s =
+  (case s of
+    Spc x \<Rightarrow> x
+    | _ \<Rightarrow> Inl (Seq.Sskip))" (* NB choice of which sskip is arbitrary here *)
+
+definition cond_trans :: "syn \<Rightarrow> cond_syn'" where
+"cond_trans s =
+  (case s of
+    Scond x \<Rightarrow> x
+    | _ \<Rightarrow> Sskip_cond)"
+
+term "prod_l (id_l) ((snd_l (snd_l id_l)))"
+
+definition printcalcseq_sem_l :: "syn \<Rightarrow> state \<Rightarrow> state" where
+"printcalcseq_sem_l =
+  l_map2' printcalc_trans
+     (prod_l id_l (snd_l id_l))
+     (pcomp print_calc_seq_lc)"
+
+definition imp_prio :: "(syn' \<Rightarrow> nat)" where
+"imp_prio x =
+(case x of
+    Sskip \<Rightarrow> 0
+    | _ \<Rightarrow> 2)"
+  
+
+(* is reassociation going to be a problem? *)
+(* also - we need to match on syntax I think?
+don't always want inc2 *)
+definition imp_sem_l :: "syn \<Rightarrow> state \<Rightarrow> state" where
+"imp_sem_l =
+  l_map2' imp_trans
+    (prod_l (prod_l (option_l (triv_l id_l))
+                    (prod_l (prio_l_case_inc imp_prio (option_l (triv_l id_l)))
+                            (prio_l_case_inc imp_prio (option_l (triv_l id_l)))))
+            (fst_l (prio_l_keep (option_l (triv_l id_l)))))
+    imp_ctl_sem"
+
+definition cond_sem_l :: "syn \<Rightarrow> state \<Rightarrow> state" where
+"cond_sem_l =
+  l_map2' cond_trans
+    (snd_l (prod_l (prio_l_inc (option_l (triv_l id_l))) 
+                   (fst_l (prio_l_keep (option_l (triv_l (id_l)))))))
+  cond_sem"
+
+definition pcs_cond_lc :: "(syn, state) langcomp" where
+"pcs_cond_lc =
+  \<lparr> Sem1 = printcalcseq_sem_l
+  , Sem2 = cond_sem_l \<rparr>"
+
+definition imp_lc :: "(syn, state) langcomp" where
+"imp_lc =
+  \<lparr> Sem1 = (pcomp pcs_cond_lc)
+  , Sem2 = imp_sem_l \<rparr>"
+
+definition sem_final :: "(syn, state) x_sem'" where
+"sem_final =
+  l_map2' id
+    (prod_fan_l (l_reverse (fst_l (prod_l (option_l (triv_l id_l))
+                                          (fst_l (prio_l_keep (option_l (triv_l (id_l)))))))) id_l)
+    (pcomp imp_lc)"
+
+
+definition gsx :: "syn gensyn \<Rightarrow> childpath \<Rightarrow> state \<Rightarrow> nat \<Rightarrow> state option" where
+"gsx =
+  gensyn_sem_exec (xsem sem_final)"
+
+definition testprog :: "syn gensyn" where 
+"testprog = G (Spc (Inl Sseq))
+              [ G (Spc (Inr (Sreset 0))) []
+              , G (Simp Sif)
+                  [ G (Scond Seqz) []
+                  , G (Spc (Inr (Sadd 1))) []
+                  , G (Spc (Inr (Sadd 2))) [] ]]"
+
+definition initial :: "state" where
+"initial =
+  (  ( Some (mdt (gs_sk testprog))
+     , (mdp 0 (Some (mdt (GRPath []))))
+     , mdp 0 (Some (mdt Down)))
+  , (mdp 0 (Some (mdt False)))
+  , (mdp 0 (Some (mdt 2)), Some (mdt [])))"
+
+
+definition testprog' :: "syn gensyn" where
+"testprog' = G (Spc (Inl Sseq)) [G (Spc (Inr (Sreset 0))) []]"
+
+
+definition initial' :: "state" where
+"initial' =
+  (  ( Some (mdt (gs_sk testprog'))
+     , (mdp 0 (Some (mdt (GRPath []))))
+     , mdp 0 (Some (mdt Down)))
+  , (mdp 0 (Some (mdt False)))
+  , (mdp 0 (Some (mdt 2)), Some (mdt [])))"
+
+term "(l_reverse (fst_l (prod_l (option_l (triv_l id_l))
+                                          (fst_l (prio_l_keep (option_l (triv_l (id_l))))))))"
+
+value [simp] "l_reverse (fst_l (prod_l (option_l (triv_l id_l))
+                                          (fst_l (prio_l_keep (option_l (triv_l (id_l)))))))
+(Spc (Inl Sseq)) initial'
+"
+
+
+value [simp] "(pcomp imp_lc) (Spc (Inl Sseq)) initial'"
+
+value "gsx testprog' [] initial' 20"
+
+value "gsx testprog [] initial 900"
+
+value "gensyn_cp_parent (G () []) []"
+
+declare [[show_types = false]]
+
+lemma what:
+  fixes x
+  assumes H : "gsx testprog' [] initial' 3 = x"
+  shows False using H
+  apply(simp add:gsx_def xsem_def testprog'_def initial'_def sem_final_def
+        prod_fan_l_def l_reverse_def fst_l_def prod_l_def option_l_def triv_l_def id_l_def
+        l_map2'_def pcomp_def imp_lc_def imp_sem_l_def pcs_cond_lc_def
+        printcalcseq_sem_l_def printcalc_trans_def
+        print_calc_seq_lc_def imp_ctl_sem_def
+        prio_l_keep_def prio_l_inc2_def prio_l_inc_def prio_l_zero_def
+        prio_l_def prio_l_const_def
+        prod_l_def fst_l_def snd_l_def
+        PrintCalcSeq.seq_sem_l_def Seq.seq_sem_l_def
+        print_calc_sem_l_def cond_sem_l_def
+        print_calc_lc_def
+        print_sem_l_def calc_sem_l_def
+        imp_trans_def print_trans_def calc_trans_def cond_trans_def seq_trans_def
+Imp.printcalc_trans_def)
+
+end
