Examples/PrintCalcSeq.thy
@@ -1,0 +1,88 @@
+theory PrintCalcSeq
+  imports PrintCalc "../MergeSemTc/Seq" "../Semantics/Gensyn_Sem"
+begin
+
+type_synonym syn = "Seq.syn + PrintCalc.syn"
+type_synonym state = "Seq.state * PrintCalc.state"
+
+definition seq_trans :: "syn \<Rightarrow> Seq.syn" where
+"seq_trans s =
+  (case s of
+  Inl s' \<Rightarrow> s'
+  | _ \<Rightarrow> Seq.Sskip)"
+
+definition printcalc_trans :: "syn \<Rightarrow> PrintCalc.syn" where
+"printcalc_trans s =
+  (case s of
+    Inr s' \<Rightarrow> s'
+   | _ \<Rightarrow> PrintCalc.Sskip)"
+
+(* problem: need different lifting behaviors
+   depending on whether we are Seq or Other (?) *)
+
+definition seq_sem_l ::
+  "syn \<Rightarrow> state \<Rightarrow> state" where
+"seq_sem_l =
+  l_map2' seq_trans
+    (fst_l (id_l)) (Seq.seq_sem_l)"
+    
+definition print_calc_sem_l ::
+  "syn \<Rightarrow> state \<Rightarrow> state" where
+"print_calc_sem_l =
+  l_map2' printcalc_trans
+    (snd_l (id_l)) (pcomp print_calc_lc)"
+
+definition print_calc_seq_lc :: "(syn, state) langcomp" where
+"print_calc_seq_lc =
+  \<lparr> Sem1 = seq_sem_l
+  , Sem2 = print_calc_sem_l \<rparr>"
+
+definition prog :: "syn gensyn" where
+"prog =
+  G (Inl Sseq) [
+    G (Inr (Sreset 0)) [],
+    G (Inr (Sadd 2)) [],
+    G (Inr (Sadd 3)) [] ]"
+
+definition prog' :: "syn gensyn" where
+"prog' =
+  G (Inl Sseq) [
+    G (Inr (Sreset 0)) [],
+    G (Inl Sseq) [G (Inr (Sadd 2)) []],
+    G (Inr (Sadd 3)) [] ]"
+
+value [simp] "pcomp print_calc_seq_lc (Inl (Sseq))
+((Some (mdt (gs_sk prog)), (mdp 0 (Some (mdt (GRPath [])))), mdp 0 (Some (mdt Down))), (mdp 0 (Some (mdt 2)), Some (mdt [])))"
+
+
+(* finally, need a way to get the childpath/lifting in and out *)
+(* we need a "fanout" lg here.
+   idea is that we are copying pieces of the product to first and second components.
+    *)
+definition sem_final :: "(syn, state) x_sem'" where
+"sem_final =
+  l_map2' id
+    (prod_fan_l (l_reverse (fst_l (prod_l (option_l (triv_l id_l))
+                                          (fst_l (prio_l_keep (option_l (triv_l (id_l)))))))) id_l)
+    (pcomp print_calc_seq_lc)"
+term "(prod_fan_l (l_reverse (fst_l (prod_l (option_l (triv_l id_l))
+                                          (fst_l (prio_l_keep (option_l (triv_l (id_l)))))))) id_l)"
+value [simp] "(l_reverse (fst_l (prod_l (option_l (triv_l id_l))
+                          (prio_l_keep (option_l (triv_l (id_l)))))))"
+
+(* TO DOS:
+- finish generalizing lifting (and lifting validation) to take syntax
+- allow for input/output states to differ (e.g. read only/read-write)
+*)
+
+
+definition gsx :: "syn gensyn \<Rightarrow> childpath \<Rightarrow> state \<Rightarrow> nat \<Rightarrow> state option" where
+"gsx =
+  gensyn_sem_exec (xsem sem_final)"
+
+value  "gsx prog [] ((Some (mdt (gs_sk prog)), (mdp 0 (Some (mdt (GRPath [])))), mdp 0 (Some (mdt Down))), (mdp 0 (Some (mdt 2)), Some (mdt []))) 90"
+
+value  "gsx prog' [] ((Some (mdt (gs_sk prog')), (mdp 0 (Some (mdt (GRPath [])))), mdp 0 (Some (mdt Down))), (mdp 0 (Some (mdt 2)), Some (mdt []))) 900"
+
+
+end
